ModularEngine/src/LogicEngine.FStar/logicEngine.fst
@@ -11,25 +11,49 @@
 // *********************************************************
 *)
 
+(* The SimpleEngine uses backwards propagation to derive all possible       *)
+(* Substitutions that will satisfy the given query. Each Substitution will  *)
+(* have an accompanying list of side conditions to be checked against the   *) 
+(* substrate(s). Only those Substitutions that pass the side conditions are *)
+(* returned                                                                 *)
 module LogicEngine
   open TypeHeaders
   open Types
   open Term 
 
-  extern reference Utilities {language="F#";
-                              dll="LogicEngine.FStar";
-                              namespace="Microsoft.Research.Dkal.LogicEngine.FStar";
-                              classname="Utilities"}
-  extern Utilities val _value_knowledge : optionFS IInfostrate -> listFS term
-  extern Utilities val _value_checkSignature : optionFS ISignatureProvider -> term -> principal -> object -> bool
-  extern Utilities val _substrateDispatcher_solve : listFS ISubstrateQueryTerm -> listFS substitution -> listFS substitution
+  extern reference Utilities {
+    language="F#";
+    dll="LogicEngine.FStar";
+    namespace="Microsoft.Research.Dkal.LogicEngine.FStar";
+    classname="Utilities"}
+  extern Utilities val _value_knowledge : optionFS IInfostrate 
+                                          -> listFS term
+  extern Utilities val _value_checkSignature : optionFS ISignatureProvider
+                                               -> term 
+                                               -> principal
+                                               -> object 
+                                               -> bool
+  extern Utilities val _substrateDispatcher_solve : listFS ISubstrateQueryTerm
+                                                    -> listFS substitution
+                                                    -> listFS substitution
 
-  val value_knowledge : option IInfostrate -> list term
-  let value_knowledge oi = PrimsListOfList (_value_knowledge (OptionOfPrimsOption oi))
-  val value_checkSignature : option ISignatureProvider -> term -> principal -> object -> bool
-  let value_checkSignature oi t p o = _value_checkSignature (OptionOfPrimsOption oi) t p o
-  val substrateDispatcher_solve : list ISubstrateQueryTerm -> list substitution -> list substitution
-  let substrateDispatcher_solve isl sl = PrimsListOfList (_substrateDispatcher_solve (ListOfPrimsList isl) (ListOfPrimsList sl))
+  val value_knowledge : option IInfostrate 
+                        -> list term
+  let value_knowledge oi = PrimsListOfList (_value_knowledge (
+                                              OptionOfPrimsOption oi))
+  val value_checkSignature : option ISignatureProvider 
+                             -> term 
+                             -> principal
+                             -> object 
+                             -> bool
+  let value_checkSignature oi t p o = _value_checkSignature 
+                                        (OptionOfPrimsOption oi) t p o
+  val substrateDispatcher_solve : list ISubstrateQueryTerm 
+                                  -> list substitution 
+                                  -> list substitution
+  let substrateDispatcher_solve isl sl = 
+    PrimsListOfList (_substrateDispatcher_solve 
+                       (ListOfPrimsList isl) (ListOfPrimsList sl))
 
   let log = ref ""
   let _freshVarId = ref 0
@@ -45,39 +69,43 @@ module LogicEngine
     match finalOutcome infon with
     | App((SaidInfon, [Const(PrincipalConstant(p)); _])) -> principal = p
     | _ -> false
-    
+   
+  (* Checks the given evidence and builds the infon that it justifies *)
   val checkJustification : option ISignatureProvider -> term -> option term
   let rec checkJustification _signatureProvider (evidence: term) = 
     match evidence with
       | App((SignatureEvidence, [Const(PrincipalConstant(ppal)); inf;
                                  Const(SubstrateConstant(signature))])) ->
           if canSign ppal inf &&
-            value_checkSignature (*!*)_signatureProvider inf ppal signature
+            value_checkSignature _signatureProvider inf ppal signature
           then
             Some inf
           else
-            (* //log.Warn("Spoofed signature {0} from {1} on {2}", signature, ppal, inf) *)
+            (* //log.Warn("Spoofed signature {0} from {1} on {2}", 
+                          signature, ppal, inf) *)
             None      
       | App((ModusPonensEvidence, [e1; e2])) ->
-          (match checkJustification _signatureProvider e1, checkJustification _signatureProvider e2 with
+          (match checkJustification _signatureProvider e1, 
+                 checkJustification _signatureProvider e2 with
              | Some i1, Some (App((ImpliesInfon, [i1'; i2]))) when i1 = i1' ->
                  Some i2
              | _ ->
-                 (* //log.Warn("Malformed modus ponens proof on {0} and {1}", e1, e2) *)
+                 (* //log.Warn("Malformed modus ponens proof on {0} and {1}",
+                               e1, e2) *)
                  None )
       | App((AndEvidence, evidences)) ->
-          let infons = collect (fun evidence ->  
-                                  match checkJustification _signatureProvider evidence with
-                                    | Some i -> [i]
-                                    | None -> []) evidences in (* Rk: F# does not need the 'in' *)
+          let infons = collect 
+            (fun evidence ->  
+               match checkJustification _signatureProvider evidence with
+                 | Some i -> [i]
+                 | None -> []) evidences in
             if length infons = length evidences then
-              Some(App(AndInfon, infons)) (* Rk: no support for |> and <| ? *)
+              Some(App(AndInfon, infons))
             else
               (* //log.Warn("Malformed conjunction proof on {0}", evidence) *)
               None
       | App((AsInfonEvidence, [SubstrateQueryTerm(query)])) ->
           if (not(isEmpty(substrateDispatcher_solve [query] [id]))) then
-            (*Some(App(AsInfon, (SubstrateQueryTerm(query)) :: [])) *) (* Rk: can't build a list as in [1], has to use 1::[] *)
             Some(App(AsInfon, [ (SubstrateQueryTerm query) ]))
           else
             (* //log.Warn("Non-true asInfon evidence at {0}", query) *)
@@ -85,114 +113,174 @@ module LogicEngine
       | ConcretizationEvidence((ev, subst)) ->
           (match checkJustification _signatureProvider ev with
              | Some generalProof -> 
-                 let concreteProof = match generalProof with
-                   | Forall _ -> instantiate generalProof subst
-                   | _ -> term_apply generalProof subst
-		 in
+                 let concreteProof = 
+                   match generalProof with
+                     | Forall _ -> instantiate generalProof subst
+                     | _ -> term_apply generalProof subst
+                 in
                    Some concreteProof
-             | None -> None) (* Rk: no need for parenthesis or 'in' in F# *)
-      | _ -> 
-          (* //log.Warn("Unhandled evidence type at {0}", evidence) *)
-	  None
+             | None -> None)
+      | _ -> (* //log.Warn("Unhandled evidence type at {0}", evidence) *)
+             None
 
-  (*open TranslationfromFStar *)(* Rk: Why can't I do TranslationfromFStar.optionFS on next line?? *)
-  let checkJustificationWrapper (s:option ISignatureProvider) (e:term) (*: optionFS term*) =
+  (*open TranslationfromFStar *)
+  (* Rk: Why can't I do TranslationfromFStar.optionFS on next line?? *)
+  let checkJustificationWrapper (s:option ISignatureProvider) (e:term) 
+    (*: optionFS term*) =
     OptionOfPrimsOption (checkJustification s e)
 
   val freshVar : typ -> var
   let freshVar (t: typ) =
-    let name0 = (Concat "SimpleLogicEngine#Var" (string_of_any (read _freshVarId))) in
+    let name0 = (Concat "SimpleLogicEngine#Var" 
+                  (string_of_any (read _freshVarId))) in
     let ret = {
       name = name0;
       typ = t} in
       (_freshVarId := (!_freshVarId) + 1);
       ret
     
-  val tryDeriveJustification : option IInfostrate -> (substitution * list ISubstrateQueryTerm) -> term 
-                            -> (term * term) -> list (substitution * (list ISubstrateQueryTerm) * term)
-  val doDeriveJustification  : option IInfostrate -> term -> (substitution * list ISubstrateQueryTerm) 
-                           -> list (substitution * (list ISubstrateQueryTerm) * term)
+  val tryDeriveJustification : 
+    option IInfostrate 
+    -> (substitution * list ISubstrateQueryTerm)
+    -> term 
+    -> (term * term)
+    -> list (substitution * (list ISubstrateQueryTerm) * term)
+  val doDeriveJustification : 
+    option IInfostrate 
+    -> term 
+    -> (substitution * list ISubstrateQueryTerm) 
+    -> list (substitution * (list ISubstrateQueryTerm) * term)
 
+  (* close to stripPrefix, also matches on the infon inf *)
   let rec tryDeriveJustification 
-      (_infostrate: option IInfostrate) (pair_subst_conds: substitution * list ISubstrateQueryTerm)
-      (pr: term) (pair_goal_inf: term * term) =
-    match pair_subst_conds with (subst, conds) -> 
-      match pair_goal_inf with (goal, inf) -> 
-        let straight = function (goal, premise) -> (* Rk: impossible to put types of goal and premise, neigher (goal:term, premise:term) nor (goal, premise) : term * term seem to work  *)
-          (match unifyFrom premise subst goal with
-             | Some s -> [(s, conds, term_apply pr s)]
-             | None -> [] ) in 
+      (_infostrate: option IInfostrate) 
+      (pair_subst_conds: substitution * list ISubstrateQueryTerm)
+        (* current substitution with associated conditions on the substrate *)
+      (pr: term(*Evidence*))
+        (* current proof *)
+      (pair_goal_inf: term(*Infon*) * term(*Infon*))
+        (* goal (= target = template) that we are trying to prove,            *)
+        (* and infon from the infostrate that we know and try to match against *)
+      : list (substitution * (list ISubstrateQueryTerm) * term(*Evidence*)) =
+    let (subst, conds) = pair_subst_conds in
+      let (goal, inf) = pair_goal_inf in
+        (* same as immediate function of stripPrefix *)
+        let straight = function 
+          (* easy case: directly try to unify the premise and the goal *)
+          (goal, premise) -> (match unifyFrom premise subst goal with
+          (* Rk: impossible to put types of goal and premise, *)
+          (* neither (goal:term, premise:term) *)
+          (* nor (goal, premise) : term * term seem to work  *)                         
+                                | Some s -> [(s, conds, term_apply pr s)]
+                                | None -> [] ) in 
           match inf with
-            | Forall((v, t)) -> (* Rk: 'as' construct not supported *)
+            | Forall((v, t)) ->
                 (match
-                   (if domainContains subst v then
-                      (match changeVarName inf subst with (newFt, s') ->
-                         t, term_apply pr s')
+                   (* idea is just (t, pr), but this ensures there is no  *)
+                   (* variable capture                                    *)
+                   (if domainContains subst v 
+                    then let (newFt, s') = changeVarName inf subst in
+                           (t, term_apply pr s')
                     else
-                      t, pr)
-		 with (i, pr) ->
-                   tryDeriveJustification _infostrate (subst, conds) pr (goal, i) ) 
+                      (t, pr))
+                 (* then just not care about the forall v and recurse     *)
+                 with (t, pr) -> tryDeriveJustification 
+                                   _infostrate (subst, conds) pr (goal, t) )
             | App((ImpliesInfon, [i1; i2])) -> 
-                let v = freshVar Evidence in (* Rk: does not support pairs or triples in the arguments *)
+                (* v is the evidence for i2; it will eventually be replaced *)
+                let v = freshVar Evidence in 
+                (* Rk: does not support pairs or triples in the arguments *)
                 let derivePremise subst_conds_goalPr_triple = 
-                  let (subst, conds, goalPr) = subst_conds_goalPr_triple in (* Rk: does not seem to be able to parenthesize this match *)
-                  let updateProof (subst_conds_premisePr_triple : substitution * (list ISubstrateQueryTerm) * term) : (substitution * (list ISubstrateQueryTerm) * term) = 
-                    let (subst, conds, premisePr) = subst_conds_premisePr_triple in
-                    let repl = App(ModusPonensEvidence, [premisePr; pr]) in (* TODO: see Builders.fs and Primitives.fs *)
-                      ((subst : substitution), 
-                       (conds : list ISubstrateQueryTerm),
-                       (term_apply goalPr (extend id v repl : substitution) : term)) in 
-                  let tmp = doDeriveJustification _infostrate i1 pair_subst_conds in
-                    (match pair_subst_conds with (subst, conds) ->
-                       map updateProof tmp
-                    )
-	        in 
-	          append
+                  let (subst, conds, goalPr) = subst_conds_goalPr_triple in
+                  let updateProof 
+                    (subst_conds_premisePr_triple : 
+                       substitution * (list ISubstrateQueryTerm) * term(*Evidence*))
+                    : (substitution * (list ISubstrateQueryTerm) * term(*Evidence*)) = 
+                    let (subst, conds, premisePr) = 
+                      subst_conds_premisePr_triple in
+                    (* premisePr is the proof of i1 ; pr is the proof of i1 => i2 *)
+                    (* then repl is a proof of i2                                 *)
+                    let repl = App(ModusPonensEvidence, [premisePr; pr]) in
+                      (* TODO: see Builders.fs and Primitives.fs *)
+                      (subst, conds,
+                        (term_apply goalPr 
+                          (extend id v repl) : term(*Evidence*))) in 
+                  let tmp = doDeriveJustification 
+                              _infostrate i1 pair_subst_conds in
+                  let (subst, conds) = pair_subst_conds in
+                  (* TODO: make sure these are the right subst and conds *)
+                    map updateProof tmp
+                in 
+                  append
+                    (* if i1 => i2 is in the infostrate, we can try to use it directly... *)
                     (straight (goal, inf))
+                    (* ... or try to use i2 and add i1 as a precondition                  *) 
                     (collect derivePremise 
-                       (tryDeriveJustification _infostrate (subst, conds) (Var v) (goal, i2))) 
+                       (tryDeriveJustification 
+                          _infostrate (subst, conds) (Var v) (goal, i2))) 
             | inf -> straight (goal, inf)
-                
-  and doDeriveJustification (_infostrate: option IInfostrate) (infon: term) (pair_subst_conds: substitution * list ISubstrateQueryTerm) = 
-    match pair_subst_conds with (subst, conds) ->
+
+  (* same as doDerive, but also carries a justification for each result *)
+  (* (except that no prefix is carried)                                 *)
+  and doDeriveJustification 
+        (_infostrate: option IInfostrate) (target: term(*Infon*))
+        (pair_subst_conds: substitution * list ISubstrateQueryTerm) 
+        : list (substitution * (list ISubstrateQueryTerm) * term(*Evidence*)) = 
+    let (subst, conds) = pair_subst_conds in
       let straight goal =
+        (* just runs tryDeriveJustification on all the JustifiedInfon of the infostrate *)
         let aux infon = 
           match infon with
             | App((JustifiedInfon, [inf; pr])) -> 
-                tryDeriveJustification _infostrate (subst, conds) pr (goal, inf)
+               tryDeriveJustification _infostrate (subst, conds) pr (goal, inf)
             | _ -> []
-	in
+        in
           collect aux (value_knowledge _infostrate)
       in
-        (match infon with
-           | App((AsInfon, [ SubstrateQueryTerm(exp) ])) ->
-               (subst, append conds (exp :: []), App(AsInfonEvidence, SubstrateQueryTerm(exp) :: [])) :: []
-           | App((AndInfon, infons)) -> (* TODO: fix the performance decrease *)
-               let parts = 
-                 (fold_left 
-                    (fun res infon ->
-                       fold_right
-                         (fun sce_triple res2 -> 
-                            let (subst, conds, evLeft) = sce_triple in
-                              append 
-				(fold_right
-                                   (fun sce_triple2 res3 ->
-                                      let (subst, conds, evRight) = sce_triple2 in
-                                        (subst, conds, 
-                                         App(AndEvidence, evLeft :: evRight :: [])) :: res3)
-                                   (doDeriveJustification _infostrate infon (subst, conds)) []
-                                ) 
-				res2
-			 ) res [])
-                    ((subst, conds, App(EmptyEvidence, [])) :: []) 
-                    infons
-		 )
-	       in 
-                 append (straight infon) []
-           | goal -> straight goal 
-        ) 
+        (match target with
+          | App((AsInfon, [ SubstrateQueryTerm(exp) ])) ->
+            (* AsInfon(...) is stored as a new side condition *)
+               [(subst, append conds [exp], 
+                 App((AsInfonEvidence, SubstrateQueryTerm(exp) :: [])))]
+                  (* Rk2: cannot change SubstrateQueryTerm(exp) :: [] to [...] *)
+          | App((AndInfon, infons)) ->(* TODO: fix the performance decrease *)
+            (* In the case of conjunction we start with the current substitution and side conditions and *)
+            (* continue accumulating these by calling recursively on each of the infons in the conjunction *)
+              let parts = 
+                (fold_left (* should be done more efficiently with a fold_right *)
+                   (fun res infon ->
+                      collect
+                        (fun sce_triple -> 
+                           let (subst2, conds2, evLeft) = sce_triple in
+                             map
+                               (fun sce_triple2 ->
+                                   let (subst3, conds3, evRight) = 
+                                     sce_triple2 in
+                                     (subst3, conds3, 
+                                       App(AndEvidence, evLeft :: [evRight])))
+                                       (* Bug? I think if evLeft=App(AndEvidence, lLeft),
+                                          the evidence here should be App(AndEvidence, lLeft :: [evRight])
+                                          otherwise it should just be App(AndEvidence, evLeft :: [evRight])
+                                        *)
+                               (doDeriveJustification 
+                                   _infostrate infon (subst2, conds2))     
+                        ) res)
+                   [(subst, conds, App(EmptyEvidence, []))]
+                   infons)
+              in 
+                append
+                  (* to prove an and, we can prove the and(...) directly...*)
+                  (straight target)
+                  (* ... or prove each subterm one by one *)
+                  parts
+          | goal -> straight goal)
   
-  val unifyAndSimpl : option substitution -> list (term * term) -> option substitution
+  val unifyAndSimpl : option substitution 
+                      -> list (term * term)
+                      -> option substitution
+  (* Given a substitution s, tries to build a more precise substitution  *)
+  (* that unifies all the pairs of terms in ts.                          *)
+  (* Returns None if failed.                                             *)
   let rec unifyAndSimpl (s: option substitution) (ts: list (term * term)) = 
     match ts with
       | [] -> s
@@ -201,82 +289,171 @@ module LogicEngine
              | None -> None
              | Some s -> unifyAndSimpl (unifyFrom a s b) ts)
 
-  val stripPrefix : substitution -> list (term * term) -> list term -> (term -> term) 
-                -> ((list term) * term) -> term -> ref (list (substitution * list term)) -> unit
-  let rec stripPrefix subst prefixUnif preconds suff t template res = 
-    let immediate = function
-      | ([], i) ->
-          (match unifyAndSimpl (Some subst) ((template, i) :: prefixUnif) with
+  val stripPrefix : substitution 
+                    -> list (term * term)
+                    -> list term
+                    -> (term -> term) 
+                    -> ((list term) * term)
+                    -> term 
+                    -> ref (list (substitution * list term)) 
+                    -> unit
+
+  (* Tries to prove template using infon (=snd(pairPrefixInfon)), an infon *)
+  (* from the infostrate. prefixUnif is a list of terms whose unification  *)
+  (* has been delayed; preconds is a list of preconditions to be fulfilled,*)
+  (* prefix (=fst(pairPrefixInfon)) and suff deal with the said prefixes.  *)
+  (* The result is added to the list res through a side effect.            *)
+  let rec stripPrefix (subst:substitution)
+    (prefixUnif:list (term(*Principal|Infon*) * term(*Principal|Infon*)))
+      (* a prefix of pairs of terms to be unified;     *)
+      (* can be pairs of Principals or pairs of Infons *)
+    (preconds:list term(*Infon*))
+      (* preconditions already calculated and carried over in rec calls *)
+    (suff:term(*Infon*) -> term(*Infon*)) 
+      (* suff is a function that takes an infon and adds a prefix in front *)
+      (* of it, of the form "p1 said p2 said [.]"                          *)
+      (* it starts empty but plays with the prefix and the infon like this:*)
+      (* if suff adds "p1; p2; p3", prefix is "p4; p5" and infon is "p4 said I"*)
+      (* then it is the same as suff adding "p1; p2; p3; p4", prefix being "p5"*)
+      (* and infon being I; that's what the SaidInfon recursive call is about. *)
+    (pairPrefixInfon:((list term(*Principal*)) * term(*Infon*))) 
+      (* a prefix pref and an infon i from the infostrate,   *)
+      (* that we are trying to match template to             *)
+      (* The prefix comes from the initial target, and is the*)
+      (* prefix to which the infon's prefix SHOULD match     *)
+    (template:term(*Infon*))
+      (* the template = target *)
+    (res:ref (list (substitution * list term(*Infon*)))) : unit = 
+      (* the result that will be updated through side effects                *)
+      (* it consists of a list of substitution and, associated with each     *)
+      (* substitution, a list of preconditions that need to be fulfilled for *)
+      (* this substitution to be a valid solution to the target              *)
+    let immediate = function (* always called on pairPrefixInfon *)
+      | ([], infon) ->
+        (* we try to directly match template to the infon i from the infostrate; *)
+        (* if we can fulfill all the other conditions in prefixUnif, that's a    *)
+        (* solution to add to res.                                               *)
+          (match unifyAndSimpl (Some subst) ((template, infon) :: prefixUnif) with
              | Some subst ->
                  (res := ((subst, preconds) :: (!res)))
              | None -> ())
       | _ -> () in 
-      (match t with
-         | ((t1 :: pref), App((SaidInfon, [t2;i]))) -> (* Rk: type annotation on t1 not supported *)
+      (match pairPrefixInfon with
+         | ((t1 :: pref), App((SaidInfon, [t2;i]))) -> 
+           (* if the infon from the infostrate is a said, we try to match it     *)
+           (* against t1, the head of the prefix                                 *)
+           (* only two cases where suff is changed *)
              (match unifyFrom t1 subst t2 with
                 | Some subst -> 
                     stripPrefix subst prefixUnif preconds 
-                      (fun j -> suff (App(SaidInfon, [t2;j]))) (pref, i) template res
-                | None ->
+                      (fun j -> suff (App(SaidInfon, [t2;j])))
+                      (pref, i) template res
+                | None -> (* Q: I think this case in unnecessary:              *)
+                          (* if the call to unifyFrom returned no solution     *)
+                          (* there is no reason why it would have a solution   *)
+                          (* later. On all the pairs of prefixUnif, eventually *)
+                          (* unifyFrom will be called (in unifyAndSimpl).      *)
                     stripPrefix subst ((t1, t2) :: prefixUnif)
-                      preconds (fun j -> suff (App(SaidInfon, [t2;j]))) (pref, i) template res) 
+                      preconds (fun j -> suff (App(SaidInfon, [t2;j])))
+                      (pref, i) template res) 
          | (pref, App((AndInfon, infons))) ->
+           (* if an and is in the infostrate, we can use any of it subterms as *)
+           (* given. Q: we never try to use the and directly?                  *)
+           (* A: probably because we already stripped down the target in       *)
+           (* doDerive                                                         *)
              iterate (fun infon -> 
-                        stripPrefix subst prefixUnif preconds suff (pref, infon) template res) infons
-         | (pref, App((ImpliesInfon, a :: b :: []))) ->
-             immediate t;
-             stripPrefix subst prefixUnif (suff a :: preconds) suff (pref, b) template res
+                        stripPrefix subst prefixUnif preconds suff 
+                          (pref, infon) template res) infons
+         | (pref, App((ImpliesInfon, [a; b]))) ->
+           (* if a => b is in the infostrate, we can try to use it directly... *)
+             immediate pairPrefixInfon;
+           (* ... or try to use b and add a as a precondition                  *) 
+             stripPrefix subst prefixUnif (suff a :: preconds) suff 
+                                          (* only place where suff is actually used *)
+               (pref, b) template res
          | (pref, Var v) when domainContains subst v ->
-             stripPrefix subst prefixUnif preconds suff (pref, subst_apply subst v) template res
-         | t -> immediate t)
+           (* If a variable is part of the current substitution it is applied *)
+           (* and we call recursively *)
+             stripPrefix subst prefixUnif preconds suff 
+               (pref, subst_apply subst v) template res
+         | pairPrefixInfon -> immediate pairPrefixInfon)
 
-  let infonsWithPrefix (_infostrate: option IInfostrate) (subst: substitution) (pref: list term) (template: term) =
+  (*   Heart #1 of backwards chaining                                        *)
+  (* Given a current Substitution, a prefix (list of principal ITerms) and   *)
+  (* a target infon ITerm to derive, this method will return a list of       *)
+  (* Substitutions that satisfy the given template, each of which will have a*)
+  (* list of preconditions (infon ITerms) that need to be verified in order  *)
+  (* for that Substitution to be a real solution                             *)
+  let infonsWithPrefix (_infostrate: option IInfostrate) (subst: substitution)
+                       (pref: list term(*Principal*)) (target: term(*Infon*)) 
+                       : list (substitution * list term(*Infon*)) =
     let res = ref [] in
-      iterate (fun k -> stripPrefix subst [] [] (fun x -> x) (pref, k) template res) 
-        (value_knowledge _infostrate);
+      iterate (fun k -> stripPrefix subst [] [] (fun x -> x) 
+                         (pref, k) target res)
+              (value_knowledge _infostrate (* : list term(*Infon*)*));
       !res
     
-  val doDerive : option IInfostrate -> list term -> (substitution * list ISubstrateQueryTerm) -> term 
-              -> list (substitution * list ISubstrateQueryTerm)
-  val checkOne : option IInfostrate -> ( ((substitution * list ISubstrateQueryTerm) * list term )
-              -> list (substitution * list ISubstrateQueryTerm))
+  val doDerive : option IInfostrate 
+                 -> list term 
+                 -> (substitution * list ISubstrateQueryTerm) 
+                 -> term 
+                 -> list (substitution * list ISubstrateQueryTerm)
+  val checkOne : option IInfostrate 
+                 -> ( ((substitution * list ISubstrateQueryTerm) * list term )
+                 -> list (substitution * list ISubstrateQueryTerm))
 
-  (*  Given a prefix (list of principal ITerms) a current Substitution with  *)
-  (*  side conditions (AsInfo ITerms) and a target infon ITerm to derive *)
+  (*  Given a prefix (list of principal ITerms) a current Substitution with *)
+  (*  side conditions (AsInfo ITerms) and a target infon ITerm to derive    *)
   (*  this method will recursively derive the target infon depending on its *)
   (*  structure. *)
-  let rec doDerive (_infostrate: option IInfostrate) (pref: list term) (* pref is a prefix of principals p said q said ... *) 
+  let rec doDerive (_infostrate: option IInfostrate) (pref: list term(*Principal*)) 
+      (* pref is a prefix of principals p said q said ... *) 
       (pair_subst_conds: substitution * list ISubstrateQueryTerm)
-      (infon: term) = (* infon is the target *)
-    let (subst, conds)= pair_subst_conds in  (* Rk: does not support patterns in formal parameters *)
-      match infon with
+      (target: term(*Infon*)) =
+    (* invariant: the result substitution is an extension of subst? (check it) *)
+    let (subst, conds)= pair_subst_conds in
+      match target with
         | App((AndInfon, infons)) -> 
+          (* In the case of conjunction we start with the current substitution and side conditions and *)
+          (* continue accumulating these by calling recursively on each of the infons in the conjunction *)
             (* Q: this fold_left indicates that the returned list is order insensitive *)
             fold_left (fun substs infon ->
                          collect 
                            (fun s -> doDerive _infostrate pref s infon) substs)
-              ((subst, conds) :: []) infons
+              [(subst, conds)] infons
         | App((EmptyInfon, []))-> 
-            (subst, conds) :: []
+          (* Empty infon is always satisfiable by the current substitution and side conditions *)
+            [(subst, conds)]
         | App((SaidInfon, [ppal; infon])) ->
+          (* Said infons are handled recursively by pushing the principal term into the prefix *)
             doDerive _infostrate (ppal :: pref) (subst, conds) infon
         | Var(v) when domainContains subst v ->
+          (* If a variable is part of the current substitution it is applied and we call recursively *)
             doDerive _infostrate pref (subst, conds) (subst_apply subst v)
         | App((AsInfon, [SubstrateQueryTerm(exp)])) ->
+          (* AsInfon(...) is stored as a new side condition, unless it is inside a non-empty prefix *)
             if isEmpty pref 
             then [(subst, append conds [exp])] (* Q: why not cons? seems to be order sensitive here. *)
             else failwith "asInfon(...) under prefix"
         | App((JustifiedInfon, [inf; ev])) when pref = [] ->
+          (* Justified infons are treated separately since we need to construct proofs for these *)
+          (* we only keep (subst, conds) whose associated evidence unifies with ev *)
             let unifyEv triple = 
-              let (subst', conds', pr') = triple in
-                match unifyFrom ev subst' pr' with
-                  | Some s ->                      (*                       let x = (append conds conds' : list ISubstrateQueryTerm) in *)
-                      let x = append conds conds' in 
+              let (subst', conds', ev') = triple in
+                match unifyFrom ev subst' ev' with
+                  | Some s ->
+                      let x = append conds conds' in  (* Q: are the conditions contained in conds not already contained in conds'? *)
                         [(s, x)]
-                  | None -> [] in 
-              (* ([] : list (substitution * list ISubstrateQueryTerm) )) in *)
-              collect unifyEv (doDeriveJustification _infostrate inf (subst, conds))
-        | templ ->
+                  | None -> [] in (* : list (substitution * list ISubstrateQueryTerm) *)
+              collect unifyEv 
+                (doDeriveJustification _infostrate inf (subst, conds))
+        (* Q: what about ImpliesInfon? *)
+        | target ->
+          (* For every other case we call se.InfonsWithPrefix(..) which will give us a list of *)
+          (* substitutions, each of which will have a list of infon ITerms (preconditions) that *)
+          (* need to be  satisfied in order for that substitution to be returned. This is were the *)
+          (* backwards chaining happens, since we recursively check all the preconditions one by one *)
+          (* (with checkOne) *)
             (* Rk: Bug? We really should have a nested let rec *)
             (*             let rec checkOne = function *)
             (*               | (substConds, pre :: pres) ->  *)
@@ -286,45 +463,60 @@ module LogicEngine
             collect 
               (checkOne _infostrate) 
               (map 
-                 (fun (s, ps) -> ((s, conds), ps))
-                 (infonsWithPrefix _infostrate subst pref templ)) (*  : list (substitution * list term))) *)
-                
-and checkOne _infostrate = function
-    | (substConds, pre :: pres) ->
-        collect (fun s -> checkOne _infostrate (s, pres)) (doDerive _infostrate [] substConds pre)
-    | (substConds, []) ->
-        substConds :: []
+                 (fun (substitution, preconds) -> ((substitution, conds), preconds))
+                 (infonsWithPrefix _infostrate subst pref target)) (* : list (substitution * list term))) *)
   
-  let derive (_infostrate: option IInfostrate) (target: term) (substs: list substitution) : list substitution =
-    fold_right
-      (fun subst res ->
-	 append
-           (fold_right
-              (fun (subst, conds) res2 -> 
-                 append (substrateDispatcher_solve conds ([subst])) res2)
-              (doDerive _infostrate [] (subst, []) (target)) [])
-           res)
-      substs []
+  (*   Heart #2 of backwards chaining                                                    *)
+  (* Given the _infostrate, and a list of                                                *)
+  (* ((subst:substitution, conds:list ISubstrateQueryTerm), preconds:list Term(*Infon*)) *)
+  (* such that some target (not in the arguments) would be satisfied by subst if         *)
+  (* the conds are true in the substrate and if the preconds (preconditions) are true    *)
+  (* in the infostrate (i.e., as infons), derives each of the preconds to get a list of  *)
+  (* pairs (subst, conds), more precise than the initial one                             *)
+  (* such that subst satisfies the target if conds are true in the                       *)
+  (* substrate. Recursive on the set of preconditions.                                   *)
+  (* The preconds are poured into (subst, conds) to make it more precise                 *)
+  and checkOne _infostrate = function
+      | (substConds, precond :: preconds) ->
+        (* substConds2 is more precise than substConds: it satisfies precond             *)
+          collect (fun substConds2 -> checkOne _infostrate (substConds2, preconds)) 
+            (doDerive _infostrate [] substConds precond)
+      | (substConds, []) ->
+          [substConds]
+  
+  (* Obtain a list of Substitution with accompanying side conditions (AsInfon *)
+  (* ITerms) [call to doDerive]. Then return only those Substitutions that    *)
+  (* satisfy all their side conditions [call to substrateDispatcher_solve].   *)
+  let derive (_infostrate: option IInfostrate) (target: term(*Infon*)) 
+             (substs: list substitution) : list substitution =
+    collect
+      (fun subst ->
+         (collect
+            (fun (subst, conds) -> 
+               (substrateDispatcher_solve conds [subst]))
+            (doDerive _infostrate [] (subst, []) target)))
+      substs
       
-  let deriveWrapper (_i: option IInfostrate) (t: term) (s: list substitution) (*: (TranslationfromFStar.listFS substitution) *)=
-    (ListOfPrimsList (derive _i t s) (* : TranslationfromFStar.listFS substitution *)) (* Rk: cannot seem to annotate with type *)
+  let deriveWrapper (_i: option IInfostrate) (t: term) (s: list substitution) 
+                    (*: (TranslationfromFStar.listFS substitution) *)=
+    (ListOfPrimsList (derive _i t s)
+     (* : TranslationfromFStar.listFS substitution *)) 
+    (* Rk: cannot seem to annotate with type *)
 
   let deriveJustification 
-      (_infostrate: option IInfostrate) (target: term) (proofTemplate: term)
+      (_infostrate: option IInfostrate) (target: term(*Infon*)) (proofTemplate: term(*Evidence*))
       (substs: list substitution) : list substitution =
-    fold_right
-      (fun subst res -> 
-	 append
-           (fold_right
-              (fun (subst, conds, proof) res2 -> 
-		 append (* Note: much like derive, except we check that ...  *)
-                   (match unifyFrom proof subst proofTemplate with (* ... the proof found is compatible with the proof template requested *)
-                      | Some subst -> substrateDispatcher_solve conds [subst]
-                      | None -> [])
-		   res2)
-              (doDeriveJustification _infostrate target (subst, [])) [])
-	   res)
-      substs []
+    collect
+      (fun subst ->
+         (collect
+            (fun (subst, conds, proof) -> (* Note: much like derive, except we check that ...*)
+               (match unifyFrom proof subst proofTemplate with (* ... the proof found is compatible with the proof template requested *)
+                  | Some subst -> substrateDispatcher_solve conds [subst]
+                  | None -> []))
+            (doDeriveJustification _infostrate target (subst, []))))
+      substs
       
-  let deriveJustificationWrapper (_i: option IInfostrate) (i: term) (p: term) (s: list substitution) (*: listFS substitution*) =
+  let deriveJustificationWrapper (_i: option IInfostrate) (i: term) 
+                                 (p: term) (s: list substitution) 
+                                 (*: listFS substitution*) =
     ListOfPrimsList (deriveJustification _i i p s)
