ModularEngine/src/LogicEngine.FStar/coredkal.fst
@@ -1,0 +1,115 @@
+module CoreDKAL
+
+type principal = string
+type var = string 
+
+type constant = 
+  | Bool : bool -> constant 
+  | Principal : principal -> constant
+  | SubstrateObject : object -> constant 
+
+type typ =  
+    | Boolean : typ
+    | Infon : typ
+    | PrincipalT : typ
+    | SubstrateQuery : typ
+    | Evidence : typ
+
+type query 
+type evidence =
+  | EmptyEv : evidence
+  | SigEv : evidence
+  | MPEv : evidence
+  | AndEv : evidence
+  | AsInfonEv : evidence
+
+type infon =
+  | Variable : var -> infon
+(*   | c  *)
+(*                | forall (x:t). i  *)
+  | Empty : infon
+  | AsInfon : query -> infon
+  | And : infon -> infon -> infon
+  | Said : infon -> infon -> infon
+(*                | And i j *)
+(*                | Implies i j *)
+
+(*                | Justified i j *)
+
+
+type infostrate = list infon
+type substrate = list query
+
+
+type In :: 'a::* => 'a => list 'a => P (* Inductive definition of list membership in a constructive style *)
+
+type MkPrefix :: list infon => infon => infon => P =
+  | MkPrefix_Nil : i:infon -> MkPrefix [] i i
+  | MkPrefix_Cons : p:infon -> ps:list infon -> i:infon -> i':infon 
+                   -> MkPrefix ps i i'
+                   -> MkPrefix (p::ps) i (Said p i')
+
+type entails :: substrate => infostrate => infon => P =
+  | Entails_Emp : S:substrate -> I:infostrate -> entails S I Empty
+
+  | Entails_Hyp_Substrate : S:substrate -> I:infostrate -> q:query 
+                 -> In q S  (* Eventually, we get a signature from the DB about this fact *)
+                 -> entails S I (AsInfon q)
+
+  | Entails_And_Intro : S:substrate -> I:infostrate 
+                     -> i:infon -> i':infon
+                     -> j:infon -> j':infon 
+                     -> result:infon
+                     -> pref: list infon
+                     -> MkPrefix pref (And i j) result
+                     -> MkPrefix pref i i'
+                     -> MkPrefix pref j j'
+                     -> entails S I i' 
+                     -> entails S I j' 
+                     -> entails S I result
+
+  | Entails_And_Elim1 : S:substrate -> I:infostrate
+     -> i : infon -> i': infon
+     -> j : infon
+     -> pref : list infon 
+     -> hyp : infon
+     -> MkPrefix pref (And i j) hyp
+     -> MkPrefix pref i i'
+     -> entails S I hyp
+     -> entails S I i'
+
+
+val checkSubstrate : S:substrate -> q:query -> option (In q S)
+(* Left unimplemented for now *)
+
+type prefix = list infon
+
+val mkPrefix: pref:prefix -> i:infon -> (i':infon * dummy:(MkPrefix pref i i'){pref=[] => i=i'})
+let rec mkPrefix pref i =
+  (match pref with
+     | [] -> (i, MkPrefix_Nil i)
+     | h::t -> let (j, m) = mkPrefix t i in
+	             ((Said h j), MkPrefix_Cons h t i j m))
+
+val doDerive: S:substrate -> I:infostrate -> pref:prefix -> i:infon 
+           -> option (i':infon * MkPrefix pref i i' * entails S I i')
+let rec doDerive _S _I pref i = match i with 
+  | Empty -> 
+      (match pref with 
+         | [] -> let (j, m) = mkPrefix pref i in
+		 (* if unable to make F* prove sth, put in a runtime check *)
+			     (* if j = Empty then *)
+                   Some((j, m, Entails_Emp _S _I))
+				  (* else raise "stupid F*" *)
+         | _ -> None)
+
+  | AsInfon q -> 
+      (match pref with
+         | [] -> let (j, m) = mkPrefix pref i in
+             (match checkSubstrate _S q with 
+                | None -> None
+                | Some pf -> Some ((j, m, Entails_Hyp_Substrate _S _I q pf)))
+         | _ -> None)
+
+  | And i j -> None (*Some((,,))*)
+      
