ModularEngine/src/LogicEngine.FStar/types.fst
@@ -20,8 +20,8 @@ open TypeHeaders
   (* BasicType types *)
     | Infon : typ
     | Principal : typ
-    | SubstrateUpdate : typ
-    | SubstrateQuery : typ
+    | SubstrateUpdate : typ (* see ISubstrateUpdate.fs *)
+    | SubstrateQuery : typ (* see ISubstrateQuery.fs *)
     | Action : typ
     | Condition : typ
     | RuleT : typ
@@ -48,44 +48,59 @@ open TypeHeaders
 
   and func =
   (* from Ast.Infon/ActivePatterns.fs *)
+  (* types from Ast.Infon/Primitives.fs, function SolveFunction *)
+  (* and its use in Ast.Infon/Builders.fs *)
     (* Rule: <condition> do <action> *)
-    | SeqRule : func
-    | EmptyRule : func
-    | Rule : func
-    | RuleOnce : func
+    | SeqRule : func (* [RuleT;...; RuleT] -> RuleT *)
+    | EmptyRule : func (* [] -> RuleT *)
+    | Rule : func (* [Condition; Action] -> RuleT *)
+    | RuleOnce : func (* [Condition; Action] -> RuleT *)
     (* Condition *)
-    | SeqCondition : func
-    | EmptyCondition : func
-    | WireCondition : func (* upon in concrete syntax *)
-    | KnownCondition : func (* if in concrete syntax *)
+    | SeqCondition : func (* [Condition;...; Condition] -> Condition *)
+    | EmptyCondition : func (* [] -> Condition *)
+    | WireCondition : func (* [Infon; Principal] -> Condition *)
+      (* upon in concrete syntax *)
+    | KnownCondition : func (* [Infon] -> Condition *)
+      (* if in concrete syntax *)
     (* Action *)
-    | SeqAction : func
-    | EmptyAction : func
-    | Send : func (* ppal (destination), msg *)
-    | JustifiedSend : func (* ppal (destination), msg *)
-    | JustifiedSay : func (* ppal (destination), msg *)
-    | Learn : func
-    | Forget : func
-    | Install : func (* add a rule to set of rules *)
-    | Uninstall : func (* regarding a rule *)
-    | Apply : func (* of substrateUpdateTerm // apply this update to the substrate *)
-    | Drop : func (* regarding an infon that came in as a message *)
+    | SeqAction : func (* [Action;...; Action] -> Action *)
+    | EmptyAction : func (* [] -> Action *)
+    | Send : func (* [Principal; Infon] -> Action *)
+      (* ppal (destination), msg *)
+    | JustifiedSend : func (* [Principal; Infon] -> Action *)
+      (* ppal (destination), msg *)
+    | JustifiedSay : func (* [Principal; Infon] -> Action *)
+      (* ppal (destination), msg *)
+    | Learn : func (* [Infon] -> Action *)
+    | Forget : func (* [Infon] -> Action *)
+    | Install : func (* [RuleT] -> Action *)
+      (* add a rule to set of rules *)
+    | Uninstall : func (* [RuleT] -> Action *)
+    | Apply : func (* [SubstrateUpdate] -> Action *)
+      (* of substrateUpdateTerm // apply this update to the substrate *)
+    | Drop : func (* [Infon] -> Action *)
+      (* regarding an infon that came in as a message *)
     (* Infon *)
-    | EmptyInfon : func
-    | AsInfon : func (* of substrateQueryTerm *)
-    | AndInfon : func (* may be easier to consider just binary case *)
-    | ImpliesInfon : func (* infon, infon *)
-    | SaidInfon : func (* ppal (sender), msg *)
-    | JustifiedInfon : func (* infon, evidence *)
+    | EmptyInfon : func (* [] -> Infon *)
+    | AsInfon : func (* [SubstrateQuery] -> Infon *)(* of substrateQueryTerm *)
+    | AndInfon : func (* [Infon; ...; Infon] -> Infon *)
+      (* may be easier to consider just binary case *)
+    | ImpliesInfon : func (* [Infon; Infon] -> Infon *)
+    | SaidInfon : func (* [Principal; Infon] -> Infon *)
+      (* ppal (sender), msg *)
+    | JustifiedInfon : func (* [Infon; Evidence] -> Infon *)
     (* Evidence *)
-    | EmptyEvidence : func
-    | SignatureEvidence : func (* ppal, term, int *)
+    | EmptyEvidence : func (* [] -> Evidence *)
+    | SignatureEvidence : func (* [Principal; Infon; Int32] -> Evidence *)
+      (* ppal, term, int *)
       (* might want to change the third type to dsig, signature for .Net *)
-    | ModusPonensEvidence : func
-    | AndEvidence : func
-    | AsInfonEvidence : func (* of substrateQueryTerm *)
+    | ModusPonensEvidence : func (* [Evidence; Evidence] -> Evidence *)
+    | AndEvidence : func (* [Evidence;... ; Evidence] -> Evidence *)
+    | AsInfonEvidence : func (* [SubstrateQuery] -> Evidence *)
+      (* of substrateQueryTerm *)
+    (* Relations defined by the writer of the policy *)
     | RelationInfon (*of relationInfon*) : relationInfon -> func
-    (* no active pattern for it, base case for infons *)
+      (* no active pattern for it, base case for infons *)
 
   and substitution = Dictionary var term 
   (* wrap the functions of dictionary used inside
